src/FairSim.v
@@ -16,13 +16,12 @@ Set Implicit Arguments.
 Section SIM.
 
   Context {Ident: ID}.
-  Variable wf: WF.
-
-  (* Definition stuck_idx (m: imap) (j: id) := le (m j) 0. *)
+  Variable wfs: WF.
+  Variable wft: WF.
 
   Inductive _sim
-            (sim: forall R0 R1 (RR: R0 -> R1 -> Prop), bool -> (imap wf) -> bool  -> (imap wf) -> (@state _ R0) -> (@state _ R1) -> Prop)
-            {R0 R1} (RR: R0 -> R1 -> Prop) (p_src: bool) (m_src: imap wf) (p_tgt: bool) (m_tgt: imap wf) :
+            (sim: forall R0 R1 (RR: R0 -> R1 -> Prop), bool -> (imap wfs) -> bool  -> (imap wft) -> (@state _ R0) -> (@state _ R1) -> Prop)
+            {R0 R1} (RR: R0 -> R1 -> Prop) (p_src: bool) (m_src: imap wfs) (p_tgt: bool) (m_tgt: imap wft) :
     (@state _ R0) -> (@state _ R1) -> Prop :=
   | sim_ret
       r_src r_tgt
@@ -84,9 +83,9 @@ Section SIM.
     _sim sim RR p_src m_src p_tgt m_tgt (trigger Undefined >>= ktr_src0) itr_tgt0
   .
 
-  Lemma sim_ind (r: forall R0 R1 (RR: R0 -> R1 -> Prop), bool -> (imap wf)  -> bool -> (imap wf) -> (@state _ R0) -> (@state _ R1) -> Prop)
+  Lemma sim_ind (r: forall R0 R1 (RR: R0 -> R1 -> Prop), bool -> (imap wfs)  -> bool -> (imap wft) -> (@state _ R0) -> (@state _ R1) -> Prop)
         R0 R1 (RR: R0 -> R1 -> Prop)
-        (P: bool -> (imap wf)  -> bool -> (imap wf) -> (@state _ R0) -> (@state _ R1) -> Prop)
+        (P: bool -> (imap wfs)  -> bool -> (imap wft) -> (@state _ R0) -> (@state _ R1) -> Prop)
         (RET: forall
             p_src m_src p_tgt m_tgt
             r_src r_tgt
@@ -159,7 +158,7 @@ Section SIM.
     { eapply UB; eauto. }
   Qed.
 
-  Definition sim: forall R0 R1 (RR: R0 -> R1 -> Prop), bool -> (imap wf)  -> bool -> (imap wf) -> (@state _ R0) -> (@state _ R1) -> Prop := paco9 _sim bot9.
+  Definition sim: forall R0 R1 (RR: R0 -> R1 -> Prop), bool -> (imap wfs)  -> bool -> (imap wft) -> (@state _ R0) -> (@state _ R1) -> Prop := paco9 _sim bot9.
 
   Lemma sim_mon: monotone9 _sim.
   Proof.
@@ -182,7 +181,7 @@ Section SIM.
   Hint Resolve cpn9_wcompat: paco.
 
   Lemma sim_ind2 R0 R1 (RR: R0 -> R1 -> Prop)
-        (P: bool -> (imap wf)  -> bool -> (imap wf) -> (@state _ R0) -> (@state _ R1) -> Prop)
+        (P: bool -> (imap wfs)  -> bool -> (imap wft) -> (@state _ R0) -> (@state _ R1) -> Prop)
         (RET: forall
             p_src m_src p_tgt m_tgt
             r_src r_tgt
@@ -256,13 +255,14 @@ Section SIM.
   (*********************** upto ***********************)
   (****************************************************)
 
-  Hypothesis WFTR: Transitive wf.(lt).
+  Hypothesis WFSTR: Transitive wfs.(lt).
+  Hypothesis WFTTR: Transitive wft.(lt).
 
   Variant sim_imap_ctxL
-          (sim: forall R0 R1: Type, (R0 -> R1 -> Prop) -> bool -> (imap wf) -> bool -> (imap wf) -> state -> state -> Prop)
+          (sim: forall R0 R1: Type, (R0 -> R1 -> Prop) -> bool -> (imap wfs) -> bool -> (imap wft) -> state -> state -> Prop)
           R0 R1 (RR: R0 -> R1 -> Prop)
     :
-    bool -> (imap wf) -> bool -> (imap wf) -> (@state _ R0) -> (@state _ R1) -> Prop :=
+    bool -> (imap wfs) -> bool -> (imap wft) -> (@state _ R0) -> (@state _ R1) -> Prop :=
     | sim_imap_ctxL_intro
         msrc0 msrc1 mtgt psrc ptgt st_src st_tgt
         (SIM: @sim _ _ RR psrc msrc1 ptgt mtgt st_src st_tgt)
@@ -284,8 +284,8 @@ Section SIM.
     { econs. i. specialize (SIM x). des. eapply IH. eauto. }
     { econs. des. esplits.
       2:{ eapply IH. reflexivity. }
-      clear - WFTR FAIR IMAP. unfold fair_update, soft_update in *. i. specialize (FAIR i). specialize (IMAP i). des_ifs.
-      - unfold le in IMAP. des. rewrite <- IMAP; auto. eapply WFTR; eauto.
+      clear - WFSTR FAIR IMAP. unfold fair_update, soft_update in *. i. specialize (FAIR i). specialize (IMAP i). des_ifs.
+      - unfold le in IMAP. des. rewrite <- IMAP; auto. eapply WFSTR; eauto.
       - eapply WF_le_Trans; eauto.
     }
     { econs. i. specialize (SIM m_tgt0). eapply SIM in FAIR. des. eauto. }
@@ -298,10 +298,10 @@ Section SIM.
 
 
   Variant sim_imap_ctxR
-          (sim: forall R0 R1: Type, (R0 -> R1 -> Prop) -> bool -> (imap wf) -> bool -> (imap wf) -> state -> state -> Prop)
+          (sim: forall R0 R1: Type, (R0 -> R1 -> Prop) -> bool -> (imap wfs) -> bool -> (imap wft) -> state -> state -> Prop)
           R0 R1 (RR: R0 -> R1 -> Prop)
     :
-    bool -> (imap wf) -> bool -> (imap wf) -> (@state _ R0) -> (@state _ R1) -> Prop :=
+    bool -> (imap wfs) -> bool -> (imap wft) -> (@state _ R0) -> (@state _ R1) -> Prop :=
     | sim_imap_ctxR_intro
         msrc mtgt0 mtgt1 psrc ptgt st_src st_tgt
         (SIM: @sim _ _ RR psrc msrc ptgt mtgt1 st_src st_tgt)
@@ -324,8 +324,8 @@ Section SIM.
     { econs. des. esplits; eauto. }
     { econs. i. hexploit SIM.
       2:{ i; des. eapply IH. reflexivity. }
-      clear - WFTR IMAP FAIR. unfold fair_update, soft_update in *. i. specialize (IMAP i). specialize (FAIR i). des_ifs.
-      - unfold le in IMAP. des. rewrite <- IMAP; auto. eapply WFTR; eauto.
+      clear - WFTTR IMAP FAIR. unfold fair_update, soft_update in *. i. specialize (IMAP i). specialize (FAIR i). des_ifs.
+      - unfold le in IMAP. des. rewrite <- IMAP; auto. eapply WFTTR; eauto.
       - eapply WF_le_Trans; eauto.
     }
     { clarify. econs; eauto. eapply rclo9_clo_base. econs; eauto. }
@@ -337,8 +337,8 @@ Section SIM.
 
 
   Variant sim_indC
-          (sim: forall R0 R1: Type, (R0 -> R1 -> Prop) -> bool -> (imap wf) -> bool -> (imap wf) -> (@state _ R0) -> (@state _ R1) -> Prop)
-          R0 R1 (RR: R0 -> R1 -> Prop) (p_src: bool) (m_src: imap wf) (p_tgt: bool) (m_tgt: imap wf)
+          (sim: forall R0 R1: Type, (R0 -> R1 -> Prop) -> bool -> (imap wfs) -> bool -> (imap wft) -> (@state _ R0) -> (@state _ R1) -> Prop)
+          R0 R1 (RR: R0 -> R1 -> Prop) (p_src: bool) (m_src: imap wfs) (p_tgt: bool) (m_tgt: imap wft)
     :
     (@state _ R0) -> (@state _ R1) -> Prop :=
     | sim_indC_ret
@@ -432,10 +432,10 @@ Section SIM.
 
 
   Variant sim_progress_ctx
-          (sim: forall R0 R1: Type, (R0 -> R1 -> Prop) -> bool -> (imap wf) -> bool -> (imap wf) -> state -> state -> Prop)
+          (sim: forall R0 R1: Type, (R0 -> R1 -> Prop) -> bool -> (imap wfs) -> bool -> (imap wft) -> state -> state -> Prop)
           R0 R1 (RR: R0 -> R1 -> Prop)
     :
-    bool -> (imap wf) -> bool -> (imap wf) -> (@state _ R0) -> (@state _ R1) -> Prop :=
+    bool -> (imap wfs) -> bool -> (imap wft) -> (@state _ R0) -> (@state _ R1) -> Prop :=
     | sim_progress_intro
         msrc mtgt psrc0 psrc1 ptgt0 ptgt1 st_src st_tgt
         (SIM: @sim _ _ RR psrc1 msrc ptgt1 mtgt st_src st_tgt)
